Change exp_rel and prove MkTick

compiler/backend/proofs/thunk_subst_untickProofScript.sml
@@ -89,9 +89,42 @@ Inductive exp_rel:
      v_rel (Atom x) (Atom x)) ∧
 [v_rel_DoTick:]
   (∀v w.
-     v_rel v w ⇒
+     v_rel v w ∧
+     properThunk v ⇒
        v_rel (DoTick v) w)
 End
+
+Theorem v_rel_def[simp]:
+  (∀s vs.
+     v_rel (Constructor s vs) w =
+       ∃ws. w = Constructor s ws ∧
+            LIST_REL v_rel vs ws) /\
+  (∀s x.
+     v_rel (Closure s x) w =
+       ∃y. w = Closure s y ∧
+           exp_rel x y) ∧
+  (∀f n.
+     v_rel (Recclosure f n) w =
+       ∃g. w = Recclosure g n ∧
+           LIST_REL (λ(f,x) (g,y). f = g ∧ exp_rel x y) f g) ∧
+  (∀x.
+     v_rel (Thunk (INR x)) w =
+       ∃y. w = Thunk (INR y) ∧
+           exp_rel x y) ∧
+  (∀v w.
+     v_rel (Thunk (INL v)) w =
+       ∃u. w = Thunk (INL u) ∧
+       v_rel v u) ∧
+  (∀x.
+     v_rel (Atom x) w =
+       (w = Atom x)) ∧
+  (∀v w.
+     v_rel (DoTick v) w =
+       (v_rel v w ∧
+       properThunk v))
+Proof
+  rw [] \\ rw [Once exp_rel_cases]
+QED
 
 Theorem exp_rel_subst:
   ∀vs x ws y.
@@ -187,195 +220,53 @@ Proof
   \\ ho_match_mp_tac exp_rel_strongind \\ rw []
 QED
 
-Definition proper_thunk_def[simp]:
-  proper_thunk (Thunk x) = (∃y. x = INR y) ∧
-  proper_thunk (Recclosure f n) =
-    (∃x. ALOOKUP (REVERSE f) n = SOME (Delay x)) ∧
-  proper_thunk _ = F
-End
-
-Theorem proper_thunk_dest_anyThunk:
-  ∀v. proper_thunk v ⇒
+Theorem properThunk_dest_anyThunk:
+  ∀v. properThunk v ⇒
     ∃x ws. dest_anyThunk v = INR (INR x, ws)
 Proof
   Induct \\ rw [] \\ simp [dest_anyThunk_def]
 QED
 
-Inductive exp_inv:
-[~Var:]
-  (∀n.
-     exp_inv (Var n)) ∧
-[~Value:]
-  (∀v.
-     v_inv v ⇒
-       exp_inv (Value v)) ∧
-[~Prim:]
-  (∀op xs.
-     EVERY exp_inv xs ⇒
-       exp_inv (Prim op xs)) ∧
-[~App:]
-  (∀f x.
-     exp_inv f ∧
-     exp_inv x ⇒
-       exp_inv (App f x)) ∧
-[~Lam:]
-  (∀s x.
-     exp_inv x ⇒
-       exp_inv (Lam s x)) ∧
-[~Letrec:]
-  (∀f x.
-     EVERY exp_inv (MAP SND f) ∧
-     exp_inv x ⇒
-       exp_inv (Letrec f x)) ∧
-[~Let:]
-  (∀s x y.
-     exp_inv x ∧
-     exp_inv y ⇒
-       exp_inv (Let s x y)) ∧
-[~If:]
-  (∀x y z.
-     EVERY exp_inv [x;y;z] ⇒
-       exp_inv (If x y z)) ∧
-[~Delay:]
-  (∀x.
-     exp_inv x ⇒
-        exp_inv (Delay x)) ∧
-[~Box:]
-  (∀x.
-     exp_inv x ⇒
-       exp_inv (Box x)) ∧
-[~Force:]
-  (∀x.
-     exp_inv x ⇒
-       exp_inv (Force x)) ∧
-[~MkTick:]
-  (∀x.
-     exp_inv x ⇒
-       exp_inv (MkTick x)) ∧
-[v_inv_Constructor:]
-  (∀s vs.
-     EVERY v_inv vs ⇒
-       v_inv (Constructor s vs)) ∧
-[v_inv_Closure:]
-  (∀s x.
-     exp_inv x ⇒
-       v_inv (Closure s x)) ∧
-[v_inv_Recclosure:]
-  (∀f n.
-     EVERY exp_inv (MAP SND f) ⇒
-       v_inv (Recclosure f n)) ∧
-[v_inv_Thunk_INR:]
-  (∀x.
-     exp_inv x ⇒
-       v_inv (Thunk (INR x))) ∧
-[v_inv_Thunk_INL:]
-  (∀v.
-     v_inv v ⇒
-       v_inv (Thunk (INL v))) ∧
-[v_inv_Atom:]
-  (∀x.
-     v_inv (Atom x)) ∧
-[v_inv_DoTick:]
-  (∀v.
-     v_inv v ∧
-     proper_thunk v ⇒
-       v_inv (DoTick v))
-End
-
-fun vapply tm =
-  let
-    val ty = List.hd (#1 (strip_fun (type_of tm)))
-             handle Empty => fail()
-    val v = variant (free_vars tm) (mk_var ("x", ty))
-    val tm = mk_comb (tm, v)
-  in
-    vapply tm
-  end
-  handle HOL_ERR _ => tm;
-
-Theorem exp_inv_def =
-  TypeBase.constructors_of “:exp”
-  |> map (curry mk_comb “exp_inv” o vapply)
-  |> map (SIMP_CONV (srw_ss()) [Once exp_inv_cases])
-  |> LIST_CONJ;
-
-Theorem v_inv_def =
-  TypeBase.constructors_of “:v”
-  |> map (curry mk_comb “v_inv” o vapply)
-  |> map (SIMP_CONV (srw_ss()) [Once exp_inv_cases])
-  |> LIST_CONJ;
-
-Theorem SUM_REL_def[simp,local] = quotient_sumTheory.SUM_REL_def;
-
-Theorem exp_inv_subst:
-  ∀vs x.
-    EVERY v_inv (MAP SND vs) ∧
-    exp_inv x ⇒
-      exp_inv (subst vs x)
+Theorem properThunk_dest_Tick:
+  ∀v. properThunk v ⇒
+    dest_Tick v = NONE
 Proof
-  ho_match_mp_tac subst_ind \\ rw []
-  >- ((* Var *)
-    gs [exp_inv_def, subst_def, EVERY_MAP, EVERY_EL]
-    \\ CASE_TAC \\ gs [exp_inv_def]
-    \\ drule_then strip_assume_tac ALOOKUP_SOME_REVERSE_EL
-    \\ first_x_assum (drule_then strip_assume_tac) \\ gs [])
-  >- ((* Prim *)
-    gs [exp_inv_def] \\ simp [subst_def]
-    \\ irule exp_inv_Prim
-    \\ gs [EVERY_MAP, EVERY_MEM])
-  >- ((* If *)
-    gs [exp_inv_def] \\ simp [subst_def]
-    \\ irule exp_inv_If \\ fs [])
-  >- ((* App *)
-    gs [exp_inv_def] \\ simp [subst_def]
-    \\ irule exp_inv_App \\ fs [])
-  >- ((* Lam *)
-    gs [exp_inv_def] \\ simp [subst_def]
-    \\ irule exp_inv_Lam
-    \\ first_x_assum irule
-    \\ gs [EVERY_MAP, EVERY_FILTER, LAMBDA_PROD, EVERY_MEM, FORALL_PROD,
-           SF SFY_ss])
-  >- ((* Let NONE *)
-    gs [exp_inv_def] \\ simp [subst_def]
-    \\ irule exp_inv_Let \\ fs [])
-  >- ((* Let SOME *)
-    gs [exp_inv_def] \\ simp [subst_def]
-    \\ irule exp_inv_Let \\ fs []
-    \\ first_x_assum irule
-    \\ gs [EVERY_MAP, EVERY_FILTER, LAMBDA_PROD, EVERY_MEM, FORALL_PROD,
-           SF SFY_ss])
-  >- ((* Letrec *)
-    gs [exp_inv_def] \\ simp [subst_def]
-    \\ irule exp_inv_Letrec
-    \\ gvs [EVERY_MAP, LAMBDA_PROD]
-    \\ first_assum (irule_at Any)
-    \\ gvs [EVERY_FILTER, LAMBDA_PROD]
-    \\ qabbrev_tac ‘P = λx. ¬MEM x (MAP FST f)’ \\ fs []
-    \\ irule_at Any EVERY_MONOTONIC
-    \\ first_assum (irule_at Any)
-    \\ simp [FORALL_PROD]
-    \\ rw [EVERY_MEM, LAMBDA_PROD, FORALL_PROD]
-    \\ first_x_assum irule
-    \\ first_assum (irule_at Any)
-    \\ gs [EVERY_MEM, FORALL_PROD, SF SFY_ss])
-  >- ((* Delay *)
-    gs [exp_inv_def, subst_def])
-  >- ((* Box *)
-    gs [exp_inv_def, subst_def])
-  >- ((* Force *)
-    gs [exp_inv_def, subst_def])
-  >- ((* Value *)
-    gs [exp_inv_def, subst_def])
-  >- ((* MkTick *)
-    gs [exp_inv_def, subst_def])
+  Induct \\ rw [] \\ simp []
 QED
+
+
+Theorem v_rel_properThunk:
+  v_rel v w ∧
+  properThunk v ⇒
+    properThunk w
+Proof
+  qsuff_tac ‘
+    (∀x y. exp_rel x y ⇒ T) ∧
+    (∀v w. v_rel v w ⇒ properThunk v ⇒ properThunk w)’
+  >- (
+    rw [SF SFY_ss])
+  \\ ho_match_mp_tac exp_rel_strongind
+  \\ rw [LIST_REL_EL_EQN, ELIM_UNCURRY]
+  \\ drule_then (qspec_then ‘REVERSE g’ mp_tac) ALOOKUP_SOME_EL_2
+  \\ impl_tac
+  >- (
+    simp [MAP_REVERSE]
+    \\ irule LIST_EQ
+    \\ gvs [EL_MAP])
+  \\ strip_tac \\ gvs [EL_REVERSE]
+  \\ qmatch_asmsub_abbrev_tac ‘EL m f’
+  \\ ‘m < LENGTH g’ by fs [Abbr ‘m’]
+  \\ first_x_assum (drule_then strip_assume_tac)
+  \\ gs [Once exp_rel_cases]
+QED
+
+Theorem SUM_REL_def[local,simp] = quotient_sumTheory.SUM_REL_def;
 
 Theorem exp_rel_eval_to:
   ∀k x y.
     exp_rel x y ∧
-    exp_inv x ∧
     eval_to k x ≠ INL Type_error ⇒
-      ∃j. ($= +++ (λv w. v_rel v w ∧ v_inv v))
+      ∃j. ($= +++ v_rel)
             (eval_to k x)
             (eval_to (k + j) y)
 Proof
@@ -383,15 +274,13 @@ Proof
   \\ qpat_x_assum ‘exp_rel _ _’ mp_tac
   >- ((* Value *)
     rw [Once exp_rel_cases]
-    \\ gs [eval_to_def, exp_inv_def]
-    \\ rw [Once exp_rel_cases])
+    \\ gs [eval_to_def])
   >- ((* Var *)
     rw [Once exp_rel_cases]
     \\ gs [eval_to_def])
   >- ((* App *)
     rename1 ‘App x1 y1’
-    \\ rw [Once exp_rel_cases]
-    \\ gs [exp_inv_def]
+    \\ rw [Once exp_rel_cases] \\ gs []
     \\ rename1 ‘exp_rel x1 x2’
     \\ rename1 ‘exp_rel y1 y2’
     \\ rw [eval_to_def]
@@ -486,22 +375,20 @@ Proof
       \\ qpat_assum ‘_ = INL Diverge’ (SUBST1_TAC o SYM)
       \\ first_x_assum (irule_at Any) \\ simp []
       \\ irule_at Any exp_rel_subst
-      \\ irule_at Any exp_inv_subst
       \\ qpat_x_assum ‘v_rel v1 u1’ mp_tac
-      \\ simp [Once exp_rel_cases] \\ strip_tac \\ gvs [dest_anyClosure_def,
-                                                        v_inv_def]
+      \\ simp [Once exp_rel_cases] \\ strip_tac \\ gvs [dest_anyClosure_def]
       \\ drule_then (qspec_then ‘n’ assume_tac) LIST_REL_OPTREL
       \\ gs [OPTREL_def]
       \\ qpat_x_assum ‘exp_rel x0 _’ mp_tac
       \\ simp [Once exp_rel_cases] \\ strip_tac \\ gvs []
       \\ simp [MAP_MAP_o, LAMBDA_PROD, combinTheory.o_DEF, GSYM FST_THM,
-               EVERY2_MAP, Once exp_rel_cases, EVERY_MAP, v_inv_def]
+               EVERY2_MAP, Once exp_rel_cases, EVERY_MAP]
       \\ irule_at Any LIST_EQ
       \\ gvs [LIST_REL_EL_EQN, EL_MAP, ELIM_UNCURRY]
       \\ drule_then strip_assume_tac ALOOKUP_SOME_REVERSE_EL
       \\ gvs [EVERY_EL, EL_MAP]
       \\ last_x_assum (drule_then assume_tac)
-      \\ gs [exp_inv_def])
+      \\ gs [])
     \\ ‘∀j. eval_to (j + j1 + j2 + k) y2 = eval_to (j2 + k) y2’
       by (strip_tac
           \\ irule eval_to_subst_mono \\ gs []
@@ -522,8 +409,7 @@ Proof
           \\ qpat_x_assum ‘exp_rel x0 _’ mp_tac
           \\ rw [Once exp_rel_cases] \\ gs [])
     \\ rename1 ‘v_rel v2 u2’ \\ gs []
-    \\ ‘exp_rel (subst (w1 ++ [s1,v2]) z1) (subst (w2 ++ [s2,u2]) z2) ∧
-        exp_inv (subst (w1 ++ [s1,v2]) z1)’
+    \\ ‘exp_rel (subst (w1 ++ [s1,v2]) z1) (subst (w2 ++ [s2,u2]) z2)’
       suffices_by
         (strip_tac
          \\ first_x_assum drule
@@ -539,30 +425,28 @@ Proof
            (qspec_then ‘j1 + j2 + j3 + k - 1’ assume_tac) eval_to_subst_mono
          \\ qexists_tac ‘j3’ \\ gs [])
     \\ irule_at Any exp_rel_subst
-    \\ irule_at Any exp_inv_subst
     \\ qpat_x_assum ‘v_rel v1 u1’ mp_tac
-    \\ simp [Once exp_rel_cases] \\ strip_tac \\ gvs [dest_anyClosure_def,
-                                                      v_inv_def]
+    \\ simp [Once exp_rel_cases] \\ strip_tac \\ gvs [dest_anyClosure_def]
     \\ drule_then (qspec_then ‘n’ assume_tac) LIST_REL_OPTREL
     \\ gs [OPTREL_def]
     \\ qpat_x_assum ‘exp_rel x0 _’ mp_tac
     \\ simp [Once exp_rel_cases] \\ strip_tac \\ gvs []
     \\ simp [MAP_MAP_o, LAMBDA_PROD, combinTheory.o_DEF, GSYM FST_THM,
-             EVERY2_MAP, EVERY_MAP, Once exp_rel_cases, v_inv_def]
+             EVERY2_MAP, EVERY_MAP, Once exp_rel_cases]
     \\ irule_at Any LIST_EQ
     \\ gvs [LIST_REL_EL_EQN, EL_MAP, ELIM_UNCURRY]
     \\ drule_then strip_assume_tac ALOOKUP_SOME_REVERSE_EL
     \\ gs [EVERY_EL, EL_MAP]
     \\ last_x_assum (drule_then assume_tac)
-    \\ gs [exp_inv_def])
+    \\ gs [])
   >- ((* Lam *)
     rw [Once exp_rel_cases]
-    \\ gs [eval_to_def, exp_inv_def]
-    \\ rw [Once exp_rel_cases, v_inv_def])
+    \\ gs [eval_to_def]
+    \\ rw [Once exp_rel_cases])
   >- ((* Let NONE *)
     rename1 ‘Let NONE x1 x2’
     \\ rw [Once exp_rel_cases]
-    \\ gs [eval_to_def, exp_inv_def]
+    \\ gs [eval_to_def]
     \\ IF_CASES_TAC \\ gs []
     >- (
       qexists_tac ‘0’
@@ -617,7 +501,7 @@ Proof
   >- ((* Let SOME *)
     rename1 ‘Let (SOME n) x1 x2’
     \\ rw [Once exp_rel_cases]
-    \\ gs [eval_to_def, exp_inv_def]
+    \\ gs [eval_to_def]
     \\ IF_CASES_TAC \\ gs []
     >- (
       qexists_tac ‘0’
@@ -644,8 +528,6 @@ Proof
     \\ gs []
     \\ ‘exp_rel (subst1 n v1 x2) (subst1 n u1 y2)’
       by (irule exp_rel_subst \\ gs [])
-    \\ ‘exp_inv (subst1 n v1 x2)’
-      by (irule exp_inv_subst \\ gs [])
     \\ first_x_assum (drule_all_then (qx_choose_then ‘j2’ assume_tac))
     \\ Cases_on ‘eval_to (k - 1) (subst1 n v1 x2) = INL Diverge’ \\ gs []
     >- (
@@ -688,21 +570,19 @@ Proof
     cheat)
   >- ((* Delay *)
     rw [Once exp_rel_cases]
-    \\ gs [eval_to_def, v_inv_def, exp_inv_def]
-    \\ rw [Once exp_rel_cases])
+    \\ gs [eval_to_def])
   >- ((* Box *)
-    rw [Once exp_rel_cases] \\ gs [eval_to_def, exp_inv_def]
+    rw [Once exp_rel_cases] \\ gs [eval_to_def]
     \\ rename1 ‘exp_rel x y’
     \\ ‘eval_to k x ≠ INL Type_error’
       by (strip_tac \\ gs [])
     \\ first_x_assum (drule_all_then (qx_choose_then ‘j1’ assume_tac))
     \\ qexists_tac ‘j1’
-    \\ Cases_on ‘eval_to k x’ \\ Cases_on ‘eval_to (j1 + k) y’ \\ gs []
-    \\ rw [Once exp_rel_cases, v_inv_def])
+    \\ Cases_on ‘eval_to k x’ \\ Cases_on ‘eval_to (j1 + k) y’ \\ gs [])
   >- ((* Force *)
     rw [Once exp_rel_cases]
     \\ rename1 ‘exp_rel x y’
-    \\ gs [Once eval_to_def, exp_inv_def]
+    \\ gs [Once eval_to_def]
     \\ ‘eval_to k x ≠ INL Type_error’
       by (strip_tac \\ gs [])
     \\ simp [Once eval_to_def]
@@ -724,17 +604,16 @@ Proof
       \\ Cases_on ‘dest_anyThunk v1’ \\ gs []
       >- (
         qexists_tac ‘j1’
-        \\ qpat_x_assum ‘v_rel v1 u1’ mp_tac
-        \\ rw [Once exp_rel_cases] \\ gs [dest_anyThunk_def]
-        \\ drule_then (qspec_then ‘n’ assume_tac) LIST_REL_OPTREL
-        \\ gs [OPTREL_def]
-        \\ qpat_x_assum ‘exp_rel x0 _’ mp_tac
-        \\ rw [Once exp_rel_cases] \\ gs [])
+        \\ Cases_on ‘v1’ \\ gs [dest_anyThunk_def]
+        \\ rename1 ‘ALOOKUP (REVERSE _) s’
+        \\ drule_then (qspec_then ‘s’ assume_tac) LIST_REL_OPTREL
+        \\ gs [OPTREL_def, CaseEq "exp"])
       \\ pairarg_tac \\ gvs []
       \\ ‘∃wx1 binds1. dest_anyThunk u1 = INR (wx1, binds1)’
         by (qpat_x_assum ‘v_rel v1 u1’ mp_tac
             \\ rw [Once exp_rel_cases] \\ gs [dest_anyThunk_def]
-            \\ drule_then (qspec_then ‘n’ assume_tac) LIST_REL_OPTREL
+            \\ rename1 ‘ALOOKUP (REVERSE _) s’
+            \\ drule_then (qspec_then ‘s’ assume_tac) LIST_REL_OPTREL
             \\ gs [OPTREL_def]
             \\ qpat_x_assum ‘exp_rel x0 _’ mp_tac
             \\ rw [Once exp_rel_cases] \\ gs [])
@@ -742,7 +621,7 @@ Proof
       >- (
         qexists_tac ‘j1’
         \\ qpat_x_assum ‘v_rel v1 u1’ mp_tac
-        \\ rw [Once exp_rel_cases] \\ gvs [dest_anyThunk_def, v_inv_def]
+        \\ rw [Once exp_rel_cases] \\ gvs [dest_anyThunk_def]
         \\ drule_then (qspec_then ‘n’ assume_tac) LIST_REL_OPTREL
         \\ gs [OPTREL_def]
         \\ qpat_x_assum ‘exp_rel x0 _’ mp_tac
@@ -770,18 +649,15 @@ Proof
         \\ qexists_tac ‘0’ \\ simp []
         \\ qpat_x_assum ‘v_rel v1 u1’ mp_tac
         \\ rw [Once exp_rel_cases] \\ gvs [])
-      \\ ‘exp_rel (subst_funs binds z) (subst_funs binds1 z1) ∧
-          exp_inv (subst_funs binds z)’
+      \\ ‘exp_rel (subst_funs binds z) (subst_funs binds1 z1)’
         by (simp [subst_funs_def]
             \\ irule_at Any exp_rel_subst
-            \\ irule_at Any exp_inv_subst
             \\ simp [MAP_MAP_o, combinTheory.o_DEF, LAMBDA_PROD, GSYM FST_THM,
-                     EVERY2_MAP, EVERY_MAP, Once (CONJUNCT2 exp_rel_cases),
-                     v_inv_def]
+                     EVERY2_MAP, EVERY_MAP, Once (CONJUNCT2 exp_rel_cases)]
             \\ irule_at Any LIST_EQ
             \\ qpat_x_assum ‘v_rel v1 u1’ mp_tac
             \\ simp [Once exp_rel_cases] \\ strip_tac
-            \\ gvs [dest_anyThunk_def, v_inv_def, EL_MAP, ELIM_UNCURRY,
+            \\ gvs [dest_anyThunk_def, EL_MAP, ELIM_UNCURRY,
                     LIST_REL_EL_EQN, SF CONJ_ss]
             \\ ‘OPTREL exp_rel (ALOOKUP (REVERSE f) n) (ALOOKUP (REVERSE g) n)’
               by (irule LIST_REL_OPTREL
@@ -793,7 +669,7 @@ Proof
             \\ drule_then strip_assume_tac ALOOKUP_SOME_REVERSE_EL
             \\ gs [EVERY_EL] \\ rw []
             \\ last_x_assum (drule_then assume_tac)
-            \\ gs [EL_MAP, exp_inv_def])
+            \\ gs [EL_MAP])
       \\ first_x_assum (drule_all_then (qx_choose_then ‘j2’ assume_tac))
       \\ Cases_on ‘eval_to (k - 1) (subst_funs binds z) = INL Diverge’ \\ gs []
       >- (
@@ -820,12 +696,10 @@ Proof
       \\ qpat_x_assum ‘v_rel v1 u1’ mp_tac
       \\ rw [Once exp_rel_cases] \\ gs [])
     \\ Cases_on ‘v1’ \\ gvs []
-    \\ qpat_x_assum ‘v_rel _ _’ mp_tac
-    \\ simp [Once exp_rel_cases] \\ strip_tac \\ gs []
     \\ rename1 ‘v_rel v1 u1’
     \\ IF_CASES_TAC \\ gs []
     >- (
-      gs [v_inv_def]
+      gs []
       \\ simp [Once eval_to_def]
       \\ Cases_on ‘eval_to 0 y = INL Diverge’ \\ gs []
       >- (
@@ -840,7 +714,7 @@ Proof
       \\ drule_then assume_tac v_rel_dest_Tick \\ gs []
       \\ ‘ISR (dest_anyThunk u1)’
         by (qpat_x_assum ‘v_rel v1 u1’ mp_tac
-            \\ rw [Once exp_rel_cases] \\ gvs [dest_anyThunk_def, v_inv_def]
+            \\ rw [Once exp_rel_cases] \\ gvs [dest_anyThunk_def]
             \\ drule_then (qspec_then ‘n’ assume_tac) LIST_REL_OPTREL
             \\ gs [OPTREL_def]
             \\ qpat_x_assum ‘exp_rel x0 _’ mp_tac
@@ -849,20 +723,24 @@ Proof
       \\ pairarg_tac \\ gvs []
       \\ qexists_tac ‘0’ \\ simp []
       \\ qpat_x_assum ‘v_rel v1 _’ mp_tac
-      \\ rw [Once exp_rel_cases] \\ gvs [dest_anyThunk_def, v_inv_def]
-      \\ drule_then (qspec_then ‘n’ assume_tac) LIST_REL_OPTREL
+      \\ rw [Once exp_rel_cases] \\ gvs [dest_anyThunk_def]
+      \\ rename1 ‘ALOOKUP (REVERSE g) s’
+      \\ drule_then (qspec_then ‘s’ assume_tac) LIST_REL_OPTREL
       \\ gs [OPTREL_def]
       \\ qpat_x_assum ‘exp_rel x0 _’ mp_tac
       \\ rw [Once exp_rel_cases] \\ gvs [])
     \\ drule_then assume_tac v_rel_dest_Tick
-    \\ last_x_assum (qspec_then ‘Atom foo’ assume_tac) \\ gs [](* TODO *)
-    \\ first_assum (qspec_then ‘[]’ mp_tac o CONV_RULE SWAP_FORALL_CONV)
-    \\ simp_tac std_ss [subst_funs_def] \\ simp []
-    \\ disch_then (drule_at (Pos last))
+    \\ drule_then assume_tac properThunk_dest_Tick
+    \\ drule_then strip_assume_tac properThunk_dest_anyThunk
+    \\ drule_all_then assume_tac v_rel_properThunk
+    \\ drule_then assume_tac properThunk_dest_Tick
+    \\ drule_then strip_assume_tac properThunk_dest_anyThunk
+    \\ rename1 ‘dest_anyThunk v1 = INR (INR x1, ws1)’
+    \\ rename1 ‘dest_anyThunk u1 = INR (INR x2, ws2)’
     \\ cheat)
   >- ((* MkTick *)
     rw [Once exp_rel_cases]
-    \\ gs [Once eval_to_def, exp_inv_def]
+    \\ gs [Once eval_to_def]
     \\ simp [Once eval_to_def]
     \\ rename1 ‘exp_rel x y’
     \\ ‘eval_to k x ≠ INL Type_error’
@@ -874,17 +752,15 @@ Proof
       \\ simp [Once eval_to_def])
     \\ qexists_tac ‘j1’
     \\ Cases_on ‘eval_to k x’ \\ Cases_on ‘eval_to (j1 + k) y’ \\ gs []
-    \\ rw [Once exp_rel_cases, v_inv_def]
-    \\ cheat (* TODO this needs to be checked in the semantics for MkTick *))
+    \\ IF_CASES_TAC \\ gs [])
   >- ((* Prim *)
     cheat)
 QED
 
 Theorem exp_rel_eval:
   exp_rel x y ∧
-  exp_inv x ∧
   eval x ≠ INL Type_error ⇒
-    ($= +++ (λv w. v_rel v w ∧ v_inv v)) (eval x) (eval y)
+    ($= +++ v_rel) (eval x) (eval y)
 Proof
   simp [eval_def]
   \\ DEEP_INTRO_TAC some_intro
